Finish Collecting Semantics Proof

Uppaal_Networks/UPPAAL_Asm_AbsInt.thy
@@ -187,14 +187,62 @@ fun deepen :: "(addr * 'a) set \<Rightarrow> 'a set state_map" where
 lemma deepen_fwd: "(pc, st) \<in> flat \<Longrightarrow> st \<in> lookup (deepen flat) pc" by (simp add: states_at.intros)
 lemma deepen_bwd: "st \<in> lookup (deepen flat) pc \<Longrightarrow> (pc, st) \<in> flat" by (simp add: states_at.simps)
 
-(*fun flatten :: "'a set state_map \<Rightarrow> (addr * 'a) set" where
-  "flatten sm = {(pc, st). st \<in> lookup sm pc}"*)
-
 inductive_set flatten for sm where
   "st \<in> lookup sm pc \<Longrightarrow> (pc, st) \<in> flatten sm"
 
 lemma flatten_fwd: "st \<in> lookup deep pc \<Longrightarrow> (pc, st) \<in> flatten deep" by (simp add: flatten.intros)
-lemma flatten_bwd: "(pc, st) \<in> flatten deep \<Longrightarrow> st \<in> lookup deep pc" by (meson flatten.cases) 
+lemma flatten_bwd: "(pc, st) \<in> flatten deep \<Longrightarrow> st \<in> lookup deep pc" by (meson flatten.cases)
+
+lemma flatten_deepen: "flatten (deepen m) = m"
+proof standard
+  show "flatten (deepen m) \<subseteq> m"
+  proof standard
+    fix x assume ass: "x \<in> flatten (deepen m)"
+    from ass obtain pc st where splitx: "x = (pc, st)" using prod.exhaust_sel by blast
+    from ass this have "(pc, st) \<in> flatten (deepen m)" by blast
+    hence "st \<in> lookup (deepen m) pc" by cases
+    hence "st \<in> states_at m pc" by simp
+    thus "x \<in> m" using splitx deepen_bwd by fastforce
+  qed
+  show "m \<subseteq> flatten (deepen m)"
+  proof standard
+    fix x assume ass: "x \<in> m"
+    from ass obtain pc st where splitx: "x = (pc, st)" using prod.exhaust_sel by blast
+    have "st \<in> lookup (deepen m) pc" using ass deepen_fwd splitx by fastforce
+    from this splitx show "x \<in> flatten (deepen m)" using flatten_fwd by force
+  qed
+qed
+
+lemma deepen_flatten: "deepen (flatten m) = m"
+proof -
+  have fwd: "deepen (flatten m) \<le> m"
+    by (meson deepen_bwd flatten.cases less_eq_state_map_def subsetI)
+  have bwd: "m \<le> deepen (flatten m)"
+    by (meson deepen_fwd flatten_fwd less_eq_state_map_def subsetI)
+  from fwd bwd show ?thesis by simp
+qed
+
+lemma flatten_lift_sup: "flatten (a \<squnion> b) = flatten a \<squnion> flatten b"
+proof standard
+  show "flatten (a \<squnion> b) \<subseteq> flatten a \<union> flatten b"
+  proof standard
+    fix x assume ass: "x \<in> flatten (a \<squnion> b)"
+    from ass obtain pc st where splitx: "x = (pc, st)" using prod.exhaust_sel by blast
+    from this ass have "st \<in> lookup (a \<squnion> b) pc" using flatten_bwd by fastforce
+    hence "st \<in> lookup a pc \<or> st \<in> lookup b pc" by simp
+    hence "(pc, st) \<in> flatten a \<or> (pc, st) \<in> flatten b" using flatten_fwd by force
+    from this splitx show "x \<in> flatten a \<union> flatten b" by simp
+  qed
+  show "flatten a \<union> flatten b \<subseteq> flatten (a \<squnion> b)"
+  proof standard
+    fix x assume ass: "x \<in> flatten a \<union> flatten b"
+    from ass obtain pc st where splitx: "x = (pc, st)" using prod.exhaust_sel by blast
+    from this ass have "(pc, st) \<in> flatten a \<or> (pc, st) \<in> flatten b" by simp
+    hence "st \<in> lookup a pc \<or> st \<in> lookup b pc" using flatten_bwd by force
+    hence "st \<in> lookup (a \<squnion> b) pc" by fastforce
+    from this splitx show "x \<in> flatten (a \<squnion> b)" by (simp add: flatten_fwd)
+  qed
+qed
 
 subsection "Collecting Semantics"
 
@@ -211,18 +259,12 @@ lemma propagate_preserve: "inm \<le> propagate inm sts" by simp
 
 inductive_set stepped_to for prog ctx pc where
   "ist \<in> lookup ctx ipc
-    \<Longrightarrow> program ipc = Some op
+    \<Longrightarrow> prog ipc = Some op
     \<Longrightarrow> step op (ipc, ist) = Some (pc, st)
     \<Longrightarrow> st \<in> stepped_to prog ctx pc"
 
-(*lemma "stepped_to prog ctx pc = {st. \<exists>ipc ist op. (ist \<in> lookup ctx ipc) \<and> (program ipc = Some op) \<and> (step op (ipc, ist) = Some (pc, st))}"*)
-
 fun step_all :: "program \<Rightarrow> collect_ctx \<Rightarrow> collect_ctx" where
   "step_all prog ctx = SM (stepped_to prog ctx)"
-
-(*definition step_all :: "instr \<Rightarrow> addr \<Rightarrow> collect_state set \<Rightarrow> state set" where
-  "step_all op pc instates =
-    {outs. (\<exists>ins\<in>instates. step op (pc, ins) = Some outs)}"*)
 
 lemma step_all_correct: "flatten (step_all prog (deepen flat)) = step_all_flat prog flat"
 proof standard
@@ -231,11 +273,20 @@ proof standard
     fix x assume ass: "x \<in> flatten (step_all prog (deepen flat))"
     then obtain pc st where splitx: "x = (pc, st)" using prod.exhaust_sel by blast
     from this ass have "st \<in> lookup (step_all prog (deepen flat)) pc" using flatten_bwd by fastforce
-    hence "st \<in> stepped_to prog (deepen flat) pc" by simp
-
-    thus "x \<in> step_all_flat prog flat" using step_all_flat_eq by blast
+    hence stepped: "st \<in> stepped_to prog (deepen flat) pc" by simp
+    from this obtain ist ipc op where stuff: "ist \<in> lookup (deepen flat) ipc" "prog ipc = Some op" "step op (ipc, ist) = Some (pc, st)" by cases
+    hence bwd: "(ipc, ist) \<in> flat" by (simp add: deepen_bwd)
+    from this stuff show "x \<in> step_all_flat prog flat" using splitx step_all_flat.intros by blast
   qed
-  show "step_all_flat prog flat \<subseteq> flatten (step_all prog (deepen flat))" sorry
+  show "step_all_flat prog flat \<subseteq> flatten (step_all prog (deepen flat))"
+  proof standard
+    fix x assume ass: "x \<in> step_all_flat prog flat"
+    then obtain pc st where splitx: "x = (pc, st)" using prod.exhaust_sel by blast
+    from ass obtain ipc ist instr where stuff: "(ipc, ist) \<in> flat" "prog ipc = Some instr" "step instr (ipc, ist) = Some x" by cases
+    from stuff have "ist \<in> lookup (deepen flat) ipc" by (simp add: states_at.intros)
+    from this stuff have "st \<in> lookup (step_all prog (deepen flat)) pc" by (simp add: splitx stepped_to.intros)
+    thus "x \<in> flatten (step_all prog (deepen flat))" using splitx by (simp add: flatten_fwd)
+  qed
 qed
 
 definition error_all :: "instr \<Rightarrow> addr \<Rightarrow> collect_state set \<Rightarrow> interpret_error set" where
@@ -245,39 +296,36 @@ definition error_all :: "instr \<Rightarrow> addr \<Rightarrow> collect_state se
 fun collect_step :: "program \<Rightarrow> collect_ctx \<Rightarrow> collect_ctx" where
   "collect_step prog ctx = ctx \<squnion> step_all prog ctx"
 
+lemma collect_step_correct: "flatten (collect_step prog (deepen flat)) = collect_step_flat prog flat"
+proof -
+  have "collect_step prog (deepen flat) = deepen flat \<squnion> step_all prog (deepen flat)" by simp
+  hence "flatten (collect_step prog (deepen flat)) = flatten (deepen flat) \<squnion> flatten (step_all prog (deepen flat))" by (simp add: flatten_lift_sup flatten_deepen)
+  hence "flatten (collect_step prog (deepen flat)) = flat \<squnion> step_all_flat prog flat" using flatten_deepen step_all_correct by blast
+  thus ?thesis by (simp add: collect_step_flat_def)
+qed
+
+lemma collect_step_correct2: "flatten (collect_step prog m) = collect_step_flat prog (flatten m)"
+  using collect_step_correct deepen_flatten by metis
+
 fun collect_loop :: "program \<Rightarrow> fuel \<Rightarrow> collect_ctx \<Rightarrow> collect_ctx" where
   "collect_loop prog 0 st = st" |
   "collect_loop prog (Suc n) st = collect_loop prog n (collect_step prog st)"
 
-lemma collect_step_sound:
-  assumes "collect_step prog inctx = outctx"
-  shows "collect_step_flat prog (flatten inctx) = flatten outctx"
-proof standard
-  show "collect_step_flat prog (flatten inctx) \<subseteq> (flatten outctx::state set)"
-  proof standard
-    fix x::state obtain inpc inst where x_def: "x = (inpc, inst)" by (metis surj_pair)
-    assume "x \<in> collect_step_flat prog (flatten inctx)"
-    hence "x \<in> step_all_flat prog (flatten inctx) \<or> x \<in> flatten inctx" using collect_step_flat_def by auto
-    thus "x \<in> flatten outctx"
-    proof safe
-      assume "x \<in> step_all_flat prog (flatten inctx)"
-      show ?thesis sorry
-    next
-      assume "x \<in> flatten inctx"
-      thus ?thesis using collect_step_preserve assms sorry
-    qed
-  qed
-
-  show "flatten outctx \<subseteq> collect_step_flat prog (flatten inctx)"
-  proof standard
-    fix x 
-    show "x \<in> flatten outctx \<Longrightarrow> x \<in> collect_step_flat prog (flatten inctx)" sorry
-  qed
+lemma collect_loop_as_flat:
+  "flatten (collect_loop prog n (deepen flat)) = collect_loop_flat prog n flat"
+proof (induction n arbitrary: flat)
+  case 0 then show ?case using flatten_deepen by auto
+next
+  case (Suc n)
+  obtain flatstep where flatstep: "deepen flatstep = collect_step prog (deepen flat)" using deepen_flatten by blast
+  hence "flatten (collect_loop prog (Suc n) (deepen flat)) = flatten (collect_loop prog n (deepen flatstep))" by simp
+  from this Suc have loop: "flatten (collect_loop prog (Suc n) (deepen flat)) = collect_loop_flat prog n flatstep" by simp
+  have step: "flatstep = collect_step_flat prog flat" by (metis collect_step_correct flatstep flatten_deepen)
+  from loop step show ?case by simp
 qed
 
-(*lemma collect_step_sound:
-"collect_step prog inctx = Some outctx
-  \<Longrightarrow> outst \<in> lookup_def outctx outpc
-  \<Longrightarrow> \<exists>inpc inst instr. (inst \<in> lookup_def inctx inpc) \<and> (prog inpc = Some instr) \<and> ((step instr (inpc, inst) = Some (outpc, outst)))" sorry*)
+theorem collect_loop_correct:
+  "flatten (collect_loop prog n (deepen entries)) = {st. \<exists>entry\<in>entries. steps_upto prog n entry st}"
+  using collect_loop_as_flat collect_loop_flat_correct by blast
 
 end
